AbstractPlatform/Types.bpl
@@ -163,6 +163,15 @@ function tap_proof_op_valid_in_enclave(o : tap_proof_op_t) : bool
     o == tap_proof_op_pause
 }
 
+function tap_proof_op_valid_in_privileged (o : tap_proof_op_t) : bool
+{
+    o == tap_proof_op_compute   || o == tap_proof_op_destroy   ||
+    o == tap_proof_op_enter     || o == tap_proof_op_exit      ||
+    o == tap_proof_op_launch    || o == tap_proof_op_resume    ||
+    o == tap_proof_op_pause     
+}
+
+
 // -------------------------------------------------------------------- //
 // constants for enclaves.                                              //
 // -------------------------------------------------------------------- //
